\documentclass{article}
\usepackage[dvipdfmx]{graphicx}
\usepackage{amsmath}
\usepackage{bm}

\title{Part1a}
\date{}

\begin{document}

\maketitle

\section{Derivation of 2-body interaction}

\begin{eqnarray*}
V &=& \frac{1}{2} \sum_{p\sigma_p,q\sigma_q,r\sigma_r,s\sigma_s} <p\sigma_p,q\sigma_q|v|r\sigma_r,s\sigma_s> a_{p \sigma_p}^{\dagger} a_{q \sigma_q}^{\dagger} a_{s \sigma_s} a_{r \sigma_r} \\
 &=& \frac{1}{2} \sum_{p\sigma_p,r} <p\sigma_p,p-\sigma_p|v|r\sigma_p,r-\sigma_p> a_{p \sigma_p}^{\dagger} a_{p -\sigma_p}^{\dagger} a_{r -\sigma_p} a_{r \sigma_p} \\
 &=& \frac{1}{2} \sum_{p\sigma_p,r} (-g) a_{p \sigma_p}^{\dagger} a_{p -\sigma_p}^{\dagger} a_{r -\sigma_p} a_{r \sigma_p} \\
 &=& \frac{1}{2} \sum_{p,r} (-g) \left( \left( a_{p +}^{\dagger} a_{p -}^{\dagger} a_{r -} a_{r +}  \right) + \left( a_{p -}^{\dagger} a_{p +}^{\dagger} a_{r +} a_{r -} \right) \right) \\
 &=& \frac{1}{2} \sum_{p,r} (-g) \left( \left( a_{p +}^{\dagger} a_{p -}^{\dagger} a_{r -} a_{r +}  \right) + (-1)^2 \left( a_{p +}^{\dagger} a_{p -}^{\dagger} a_{r -} a_{r +}  \right) \right) \\
 &=& -g \sum_{p,r} a_{p +}^{\dagger} a_{p -}^{\dagger} a_{r -} a_{r +} \\
 &\equiv& -g \sum_{p,r} P_p^{+} P_r^{-}. \\
\end{eqnarray*}

\section{Commutation relation}
\subsection{useful relation}
\label{use}
\begin{eqnarray*}
[A,BC] &=& B[A,C] + [A,C]B, \\
\bigl\{ A,BC \bigr\} &=& B \bigl\{ A,C \bigr\} - \bigl\{ A,C \bigr\} B,
\end{eqnarray*}
then
\begin{eqnarray*}
[AB,CD] = A \bigl\{ B,C \bigr\} D - \bigl\{ A,C \bigr\} B D + C A \bigl\{ B,D \bigr\} - C \bigl\{ A,D \bigr\} B.
\end{eqnarray*}

\subsection{$S_z$ vs $H_0$}
By making use of the relation in sec.\ref{use}, we get
\begin{eqnarray*}
[S_z,H_0] &=& \sum_{p \sigma_p}\frac{\sigma_p}{2} \sum_{q\sigma_q} (q-1) [a_{p \sigma_p}^{\dagger} a_{p \sigma_p},a_{q \sigma_q}^{\dagger} a_{q \sigma_q}] \\
&=& \sum_{p \sigma_p}\frac{\sigma_p}{2} \sum_{q\sigma_q} (q-1) \delta_{p,q}\delta_{\sigma_p,\sigma_q} \left(  a_{p \sigma_p}^{\dagger} a_{q \sigma_q} - a_{q \sigma_q}^{\dagger}a_{p \sigma_p}  \right) \\
&=& \sum_{p \sigma_p}\frac{\sigma_p}{2} (p-1) \left(  a_{p \sigma_p}^{\dagger} a_{p \sigma_p} - a_{p \sigma_p}^{\dagger}a_{p \sigma_p}  \right) \\
&=& 0.
\end{eqnarray*}

\subsection{$\bm{S}^2$ vs $H_0$}
By making use of the relation in sec.\ref{use}, we get
\begin{eqnarray*}
[S_+,H_0] &=& \sum_{p \sigma_p} (p-1) [ a_{p+}^{\dagger} a_{p-} , a_{p \sigma_p}^{\dagger} a_{p \sigma_p} ] \\
&=& \sum_{p \sigma_p} (p-1) \left( - \delta_{\sigma_p +} a_{p\sigma_p}^{\dagger} a_{p-} + \delta_{\sigma_p -} a_{p +}^{\dagger} a_{p \sigma_p} \right) \\
&=& \sum_{p} (p-1) \left( -  a_{p +}^{\dagger} a_{p-} +  a_{p +}^{\dagger} a_{p -} \right) \\
&=& 0,
\end{eqnarray*}
\begin{eqnarray*}
[S_-,H_0] = \left( - [S_+,H_0] \right)^{\dagger} = 0,
\end{eqnarray*}
therefore we get
\begin{eqnarray*}
\left[ \bm{S}^2,H_0 \right] &=& [ S_z^2 + \frac{1}{2}(S_{+}S_{-} + S_{-}S_{+}) , H_0 ] \\
&=& [S_z,H_0]S_z + S_z[S_z,H_0] + \frac{1}{2} \left( [S_{+},H_0] S_{-} + S_{+} [S_{-},H_0] + [S_{-},H_0] S_{+} + S_{-} [S_{+},H_0] \right) \\
&=& 0.
\end{eqnarray*}

\subsection{$S_z$ vs $V$}
By making use of the relation in sec.\ref{use}, we get
\begin{eqnarray*}
[P_p^{+},S_z] &=& \sum_{\sigma_p} \frac{\sigma_p}{2} [a_{p+}^{\dagger} a_{p-}^{\dagger} , a_{p\sigma_p}^{\dagger} a_{p\sigma_p} ] \\
&=& \sum_{\sigma_p} \frac{\sigma_p}{2} \left( a_{p \sigma_p}^{\dagger} a_{p+}^{\dagger} \delta_{\sigma_p-} -  a_{p \sigma_p}^{\dagger} a_{p-}^{\dagger} \delta_{\sigma_p+} \right) \\
&=& \left( -\frac{1}{2}\right) a_{p -}^{\dagger} a_{p+}^{\dagger} - \left( \frac{1}{2} \right) a_{p+}^{\dagger} a_{p-}^{\dagger} \\
&=& 0,
\end{eqnarray*}
\begin{eqnarray*}
[P_p^{-},S_z] = \left( - [P_p^{+},S_z] \right)^{\dagger} = 0,
\end{eqnarray*}
therefore we get
\begin{eqnarray*}
[S_z,V] &=& -g \sum_{p,q} [S_z, P_p^{+}P_q^{-}] \\
&=& -g \sum_{p,q} \left( [S_z, P_p^{+}]P_q^{-} + P_p^{+}[S_z, P_q^{-}] \right) \\
&=& 0.
\end{eqnarray*}

\subsection{$\bm{S}^2$ vs $V$}
By making use of the relation in sec.\ref{use}, we get
\begin{eqnarray*}
[P_p^{+},S_+] &=& [a_{p+}^{\dagger}a_{p-}^{\dagger} , a_{p+}^{\dagger} a_{p-} ] \\
&=& a_{p+}^{\dagger} a_{p+}^{\dagger} \bigl\{ a_{p-}^{\dagger} , a_{p-}  \bigr\} \\
&=& 0
\end{eqnarray*}
and
\begin{eqnarray*}
[P_p^{-},S_+] &=& \left( a_{p-} a_{p+} , a_{p+}^{\dagger} a_{p-} \right) \\
&=& a_{p-}  \bigl\{ a_{p+} , a_{p+}^{\dagger}  \bigr\} a_{p-} \\
&=& 0,
\end{eqnarray*}
then
\begin{eqnarray*}
\left[ S_{+},V \right] &=& -g \sum_{p,q} [S_{+},P_p^{+}P_q^{-}] \\
&=& -g \sum_{p,q} \left( [S_{+},P_p^{+}]P_q^{-} + P_p^{+} [S_{+},P_q^{-}] \right) \\
&=& 0,
\end{eqnarray*}
\begin{eqnarray*}
\left[ S_{-},V \right] = \left( - [S_{+} , V ] \right)^{\dagger} = 0.
\end{eqnarray*}
Therefore we get
\begin{eqnarray*}
\left[ \bm{S}^2,V \right] &=& [ S_z^2 + \frac{1}{2}(S_{+}S_{-} + S_{-}S_{+}) , V ] \\
&=& [S_z,V]S_z + S_z[S_z,V] + \frac{1}{2} \left( [S_{+},V] S_{-} + S_{+} [S_{-},V] + [S_{-},V] S_{+} + S_{-} [S_{+},V] \right) \\
&=& 0.
\end{eqnarray*}


\end{document}